HoareTactics/CSLTactics.v
@@ -1,4 +1,4 @@
-Require Import GPUCSL scan_lib LibTactics Psatz CSLLemma SetoidClass Skel_lemma scan_lib.
+Require Import GPUCSL scan_lib LibTactics Psatz CSLLemma SetoidClass Skel_lemma scan_lib CodeGen.
 Notation val := Z.
 Arguments Z.add _ _ : simpl never.
 
@@ -626,7 +626,7 @@ Ltac apply_read_rule Hle Hv Hn P Res le i :=
       idtac dist i;
       assert (Hres : Res |=R R *** Res'); [sep_auto'|
       assert (Hbnd : P -> i < length arr /\ dist (s + i) = j); [simpl; prove_pure|
-      applys (>> rule_read_array' Hle Hv Hres Hn Hbnd); eauto with novars_lemma pure_lemma]]
+      applys (>> rule_read_array' Hle Hv Hres Hn Hbnd); eauto with pure_lemma]]
     end in
   let rec iter acc Res :=
     match Res with
@@ -656,7 +656,7 @@ Ltac apply_write_rule Hle Hix He Hn P Res le i :=
       idtac "apply read rule: match sarray case.";
       assert (Hres : Res |=R R *** Res'); [sep_auto'|
       assert (Hbnd : P -> i < length arr /\ dist (s + i) = j); [prove_pure|
-      applys (>> rule_write_array' Hle Hix Hres He Hn Hbnd); eauto with novars_lemma pure_lemma]]
+      applys (>> rule_write_array' Hle Hix Hres He Hn Hbnd); eauto with pure_lemma]]
     end in
   let rec iter acc Res :=
     lazymatch Res with
@@ -944,8 +944,6 @@ Proof.
   destruct HP0; eauto.
 Qed.
 
-Definition istar ls := List.fold_right Star Emp ls.
-
 Lemma conj_xs_assn st n Res P Env :
   n <> 0 ->
   conj_xs (ls_init st n (fun i => Assn (Res i) P Env)) ==
@@ -982,84 +980,6 @@ Lemma sc_v2l n (assns : Vector.t assn n) :
   Bdiv.Aistar_v assns == conj_xs (Vector.to_list assns).
 Proof.
   simpl; introv; apply sc_v2l.
-Qed.
-
-Lemma emp_unit_l P: 
-  (Emp *** P) == P.
-Proof.
-  intros s h; unfold sat_res; simpl.
-  apply emp_unit_l.
-Qed.
-
-Lemma emp_unit_r P: 
-  (P *** Emp) == P.
-Proof.
-  intros s h; unfold sat_res; simpl.
-  apply emp_unit_r.
-Qed.
-
-Lemma init_emp_emp b n :
-  istar (ls_init b n (fun _ => Emp)) == Emp.
-Proof.
-  revert b; induction n; simpl; [reflexivity|]; intros.
-  rewrite IHn.
-  rewrite emp_unit_l; reflexivity.
-Qed.
-
-Lemma ls_star b n P Q :
-  istar (ls_init b n (fun i => P i *** Q i)) ==
-  (istar (ls_init b n (fun i => P i)) *** istar (ls_init b n (fun i => Q i))).
-Proof.
-   revert b; induction n; simpl; eauto.
-   - intros; rewrite emp_unit_l; reflexivity.
-   - intros; rewrite IHn; rewrite <-!res_assoc.
-     apply res_star_proper; [reflexivity|].
-     rewrite res_CA; reflexivity.
-Qed.
-
-Lemma istar_app Ps Qs: 
-  istar (Ps ++ Qs) == (istar Ps *** istar Qs).
-Proof.
-  induction Ps; simpl; eauto.
-  rewrite emp_unit_l; reflexivity.
-  rewrite IHPs, <-res_assoc; reflexivity.
-Qed.  
-                       
-Lemma array'_ok n ptr dist vals s p :
-  (forall i, s <= i < length vals + s -> dist i < n) ->
-  istar (ls_init 0 n (fun i => array' ptr (ith_vals dist vals i s) p)) ==
-  array ptr vals p.
-Proof.
-  revert s ptr; induction vals; intros; simpl.
-  - intros s' h.
-    rewrite init_emp_emp; reflexivity.
-  - rewrite ls_star.
-    rewrite IHvals.
-    apply res_star_proper; try reflexivity.
-    lazymatch goal with
-    | [|- context [ls_init 0 n ?f]] =>
-      cutrewrite (ls_init 0 n f =
-                  (ls_init 0 (dist s) (fun _ => Emp) ++
-                  (ptr |->p (p, a)) ::
-                  ls_init ((dist s) + 1) (n - dist s - 1) (fun _ => Emp)))
-    end.
-    rewrite istar_app, init_emp_emp; simpl; rewrite init_emp_emp.
-    rewrite emp_unit_l, emp_unit_r; reflexivity.
-    specialize (H s).
-    simpl in *.
-    cutrewrite (n = (dist s) + 1 + (n - dist s - 1)); [|omega].
-    repeat rewrite ls_init_app; simpl.
-    rewrite <-app_assoc; simpl.
-    f_equal; [apply ls_init_eq'|f_equal]; eauto.
-    intros; simpl; destruct Nat.eq_dec; try omega; eauto.
-    intros; simpl; destruct Nat.eq_dec; try omega; eauto.
-    lazymatch goal with
-    | [|- _ _ ?p _ = _ _ ?q _] =>
-      cutrewrite (q = p); [|lia];
-      apply ls_init_eq';
-      intros; simpl; destruct Nat.eq_dec; try omega; eauto
-    end.
-    intros; apply H; simpl; omega.
 Qed.
 
 Lemma nseq_nth_same T i n (x : T) :
@@ -1168,89 +1088,12 @@ Ltac prove_istar_imp :=
 Ltac ls_rewrite_in Heq H :=
   erewrite ls_init_eq0 in H; [|intros; rewrite Heq; reflexivity].
 
-Lemma precise_false : precise (fun _ _ => False).
-Proof.
-  unfold precise; intros; tauto.
-Qed.
-
-Lemma precise_sat (P Q : assn) :
-  (Q |= P) -> precise P -> precise Q.
-Proof.
-  unfold precise; simpl; intros Hsat HprecP; introv.
-  intros HsatQ HsatQ' ? ? ?.
-  eapply HprecP; eauto; apply Hsat; eauto.
-Qed.
-
-Definition precise_res P :=
-  forall (h1 h2 h1' h2' : pheap) s,
-    sat_res s h1 P ->
-    sat_res s h2 P ->
-    pdisj h1 h1' ->
-    pdisj h2 h2' ->
-    phplus h1 h1' = phplus h2 h2' -> h1 = h2. 
-
-Lemma precise_assn Res P Env :
-  precise_res Res
-  -> precise (Assn Res P Env).
-Proof.
-  unfold Assn; intros.
-  eapply precise_sat; unfold sat; intros s h Hsat; sep_split_in Hsat; eauto.
-Qed.
-
-Lemma precise_star (P Q : res) : precise_res P -> precise_res Q -> precise_res (P *** Q).
-Proof.
-  unfold_conn; intros pp pq h1 h2 h1' h2' s hsat hsat' hdis hdis' heq; simpl in *.
-  destruct hsat as [ph1 [ph1' [satp1 [satq1 [Hdis1 Heq1]]]]], 
-                   hsat' as [ph2 [ph2' [satp2 [satq2 [Hdis2 Heq2]]]]].
-  destruct h1 as [h1 ?], h2 as [h2 ?]; apply pheap_eq; simpl in *; rewrite <-Heq1, <-Heq2 in *.
-  apply pdisj_padd_expand in hdis; apply pdisj_padd_expand in hdis'; eauto.
-  rewrite !padd_assoc in heq; try tauto. 
-  f_equal; destruct hdis as [hdis1 hdis2], hdis' as [hdis1' hdis2'].
-  - rewrite (pp ph1 ph2 (phplus_pheap hdis2) (phplus_pheap hdis2') s); eauto.
-  - rewrite padd_left_comm in heq at 1; try tauto.
-    rewrite (@padd_left_comm _ ph2 ph2' h2') in heq; try tauto.
-    pose proof (pdisjE2 hdis1 hdis2) as dis12; pose proof (pdisjE2 hdis1' hdis2') as dis12'.
-    rewrite (pq ph1' ph2' (phplus_pheap dis12) (phplus_pheap dis12') s); simpl in *; eauto; 
-    apply pdisj_padd_comm; eauto.
-Qed.
-
-Lemma precise_mps l v p :
-  precise_res (l |->p (p, v)).
-Proof.
-  unfold precise_res, precise; intros; simpl in *.
-  unfold sat_res in *; simpl in *; unfold_conn_all; simpl in *.
-  destruct h1 as [h1 ?], h2 as [h2 ?]; apply pheap_eq.
-  extensionality x; simpl in *; rewrite H, H0; auto.
-Qed.
-
-Lemma precise_emp :
-  precise_res Emp.
-Proof.
-  unfold precise_res, sat_res, sat; simpl.
-  intros; applys precise_emp; simpl; eauto.
-Qed.
-
-Hint Resolve precise_star precise_mps precise_emp precise_false precise_assn.
-
-Lemma precise_array l vs p: 
-  precise_res (array l vs p).
-Proof.
-  revert l; induction vs; simpl; eauto.
-Qed.
-
-Lemma precise_array' l vs q :
-  precise_res (array' l vs q).
-Proof.
-  revert l; induction vs as [|[?|] ?]; simpl; eauto.
-Qed.              
-
-Hint Resolve precise_star precise_array precise_array'.
-
 Lemma ty_var' g v ty :
   g v = ty -> typing_exp g v ty.
 Proof.
   intros; constructor; rewrite H; destruct ty; eauto.
 Qed.
+
 Ltac prove_typing_exp :=
   lazymatch goal with
   | |- typing_exp ?E (Evar ?v) _ => apply ty_var'; simpl; eauto
@@ -1258,6 +1101,7 @@ Ltac prove_typing_exp :=
   | |- typing_exp ?E (_ ?e1 ?e2) _ => constructor; prove_typing_exp
   | |- typing_exp ?E (_ ?e) _ => constructor; prove_typing_exp
   end.
+
 Ltac prove_typing_lexp :=
   match goal with |- ?g => idtac g end;
   lazymatch goal with
@@ -1271,6 +1115,7 @@ Ltac prove_typing_lexp :=
     idtac "B";
     constructor; [prove_typing_lexp | prove_typing_exp]; simpl
   end.
+
 Ltac prove_typing_bexp :=
   match goal with |- ?g => idtac g end;
   lazymatch goal with
@@ -1696,94 +1541,3 @@ Ltac simpl_nested_istar := match goal with
     rewrites (>>conj_xs_init_flatten0 n m (fun x : nat => X)) in H
   end
 end.
-
-Lemma mps_p_star loc v (p1 p2 : Qc) :
-  (0 < p1 -> p1 <= 1 -> 0 < p2 -> p2 <= 1 -> p1 + p2 <= 1 ->
-   (loc |->p (p1 + p2, v) == (loc |->p (p1, v) *** loc |->p (p2, v))))%Qc.
-Proof.
-  unfold "=="; simpl; unfold equiv_res, sat_res; simpl.
-  intros; apply pts_star_p; auto.
-Qed.
-
-Lemma array_p_star loc xs p q :
-  (0 < p -> p <= 1 -> 0 < q -> q <= 1 -> p + q <= 1 ->
-  array loc xs (p + q) == (array loc xs p *** array loc xs q))%Qc.
-Proof.
-  revert loc; induction xs; simpl; intros.
-  - rewrite emp_unit_l; reflexivity.
-  - rewrites* IHxs.
-    rewrite* mps_p_star; eauto.
-    rewrite <-!res_assoc; split; intros; repeat sep_cancel'.
-Qed.    
-
-Require Import QArith Qcanon.
-Ltac injZ_simplify :=
-  unfold injZ in *;
-  repeat rewrite Nat2Z.inj_succ in *;
-  repeat rewrite <-Z.add_1_r in *;
-  repeat rewrite inject_Z_plus in *;
-  repeat rewrite inject_Z_1 in *.
-
-Lemma QcmultQ p q : (this (p * q)%Qc == this p * this q)%Q.
-Proof.
-  unfold "*"%Qc.
-  unfold "!!"%Qc.
-  rewrite this_id.
-  apply Qred_correct.
-Qed.
-
-Lemma is_array_is_array_p_n loc xs (p : Qc) (nt : nat) :
-  (0 < p)%Qc -> (p <= 1)%Qc -> (injZ (Zn nt) * p <= 1)%Qc -> (nt <> 0)%nat -> 
-  forall st,
-    array loc xs (injZ (Z.of_nat nt) * p) == istar (ls_init st nt (fun i => array loc xs p)).
-Proof.
-  intros Hp0 Hp1 Hnp Hn0; induction nt as [|[|nt]]; intros; try omega.
-  - simpl.
-    asserts_rewrite (injZ 1 * p = p)%Qc.
-    { apply Qc_is_canon.
-      rewrite QcmultQ.
-      lra_Qc. }
-    rewrite emp_unit_r; reflexivity.
-  - remember (S nt) as nt'.
-    asserts_rewrite (Zn (S nt') = Zn nt' + 1)%Z.
-     { rewrite Nat2Z.inj_succ; omega. }
-     unfold injZ; rewrite inject_Z_plus; simpl.
-     asserts_rewrite (Q2Qc (inject_Z (Zn nt') + inject_Z 1) = injZ (Zn nt') + 1).
-     { apply Qc_is_canon.
-       unfold injZ, "+", Q2Qc.
-       rewrite !this_inv.
-       rewrite !Qred_correct.
-       reflexivity. }
-     rewrite Qcmult_plus_distr_l, Qcmult_1_l; eauto; simpl.
-Ltac Qc_to_Q :=
-  match goal with
-  | [q : Qc |- _] => destruct q; Qc_to_Q
-  | [|- _] =>
-    try applys Qc_is_canon;
-    repeat ( unfold Q2Qc, Qcmult, Qcplus, Qcdiv, Qcinv, Qclt, Qcle in *);
-    repeat (try rewrite this_inv in *; try rewrite Qred_correct in *)
-  end.
-
-     rewrite array_p_star, IHnt; [|subst nt'; unfold injZ in *; injZ_simplify; Qc_to_Q; eauto; pose proof (inject_Z_n_ge0 nt); try lra..|].
-     split; intros; eauto; repeat sep_cancel'; eauto.
-     repeat sep_cancel'.
-     assert (0 <= inject_Z (Zn nt) * this)%Q by (apply Qmult_le_0_compat; lra_Qc).
-     lra.
-     injZ_simplify.
-     Qc_to_Q.
-     lra.
-Qed.
-
-
-Lemma is_array_is_array_p_1 loc xs (nt : nat) st :
-  (nt <> 0)%nat ->
-  array loc xs 1 ==
-  istar (ls_init st nt (fun i => array loc xs (1 / (injZ (Zn nt))))).
-Proof.    
-  intros; rewrite (@one_div_n nt) at 1; eauto.
-  apply is_array_is_array_p_n; eauto;
-  unfold injZ; Qc_to_Q; destruct nt; try omega; lets: (inject_Z_Sn_gt0 nt).
-  apply Qlt_shift_div_l; lra.
-  apply Qle_shift_div_r; try lra.
-  lets Heq: Qmult_div_r; unfold Qdiv in Heq; rewrite Heq; lra.
-Qed.
